susp_security wip

theories/examples/authentikit_base_susp_security.v
@@ -3,7 +3,7 @@ From auth.rel_logic_bin Require Export model spec_rules spec_tactics interp lib 
 From auth.heap_lang Require Import gen_weakestpre.
 From auth.heap_lang.lib Require Import list serialization.
 From auth.examples Require Export authentikit_susp authenticatable_base_susp.
-From iris.base_logic.lib Require Export invariants.
+From iris.base_logic.lib Require Export invariants na_invariants.
   
 (* Section auth_serialization.
   Context `{invGS_gen hlc Σ} `{g : !GenWp Σ} (N : namespace).
@@ -212,12 +212,15 @@ Program Definition auth_deserialization : deserialization :=
   |}. *)
 
 Section authenticatable.
-  Context `{!heapGS_gen hlc Σ}.           
+  Context `{!heapGS_gen hlc Σ, !seqG Σ} (N : namespace).
+
+  Definition authSerN (v: val) : namespace := N .@ "auth_ser" .@ v.
+  Definition authValidN (v: val) : namespace := N .@ "auth_valid" .@ v.
+  Definition authCountN (v: val) : namespace := N .@ "auth_count" .@ v.
   
   Inductive evi_type : Type :=
   | tprod (t1 t2 : evi_type)
   | tsum (t1 t2 : evi_type)
-  | toption (t1 : evi_type)
   | tstring
   | tint
   | tauth.
@@ -227,28 +230,29 @@ Section authenticatable.
 
   Definition auth_is_ser_2 (v : val) (s : string) : iProp Σ :=
     ∃ (susp : loc) (h : string),
-      ⌜v = InjRV #susp⌝ ∗ susp ↦{DfracDiscarded} (InjRV #h) ∗ s_is_ser (g:=gwp_upto_bad) auth_scheme (SOMEV #h) s.
+      ⌜v = InjRV #susp⌝ ∗ susp ↦□ InjRV #h ∗ s_is_ser (g:=gwp_upto_bad) auth_scheme (SOMEV #h) s.
 
   Definition auth_is_ser_3 (v : val) (s : string) : iProp Σ :=
-    ∃ (susp : loc),
-      ⌜v = InjRV #susp⌝ ∗ s_is_ser (g:=gwp_upto_bad) auth_scheme NONEV s.
+    ∃ (susp : loc) (pid: nat), ⌜v = InjRV #susp⌝ ∗ susp ↦ (InjLV #pid) ∗ s_is_ser (g:=gwp_upto_bad) auth_scheme NONEV s.
 
-  Definition auth_is_ser (v : val) (s : string) : iProp Σ :=
-    auth_is_ser_1 v s ∨ auth_is_ser_2 v s.
+  (* Definition auth_is_ser (v : val) (s : string) : iProp Σ :=
+    auth_is_ser_1 v s ∨ auth_is_ser_2 v s. *)
+
+  Definition valid_auth_inv (susp : loc) : iProp Σ :=
+    ((∃ (h : string), susp ↦□ InjRV #h) ∨
+       (∃ (pid : nat), susp ↦ (InjLV #pid))).
 
   Definition auth_valid_val (v1 : val) : iProp Σ :=
     ∃ v, ⌜v1 = SOMEV v⌝ ∧
            ((∃ (h : string), ⌜v = InjLV #h⌝) ∨
               (∃ (susp : loc),
-                  ⌜v = InjRV #susp⌝ ∗
-                    ((∃ (h : string), susp ↦{DfracDiscarded} (InjRV #h)) ∨
-                                       (∃ (pid : nat), susp ↦ (InjLV #pid))))).
+                  ⌜v = InjRV #susp⌝ ∗ seq_inv (authValidN #susp) (valid_auth_inv susp))).
 
-  Definition auth_ser_valid_val (v : val) : iProp Σ :=
-    ((∃ (h : string), ⌜v = InjLV #h⌝) ∨
-       (∃ (susp : loc),
-           ⌜v = InjRV #susp⌝ ∗
-             (∃ (h : string), susp ↦{DfracDiscarded} (InjRV #h)))).
+  Definition auth_deser_valid_val (v1 : val) : iProp Σ :=
+    ∃ v, ⌜v1 = SOMEV v⌝ ∧
+           ((∃ (h : string), ⌜v = InjLV #h⌝) ∨
+              (∃ (susp : loc),
+                  ⌜v = InjRV #susp⌝ ∗ (∃ (pid : nat), susp ↦ (InjLV #pid)))).
              
   
   (* Fixpoint s_is_ser_ser (t : evi_type) (v : val) (s : string) : iProp Σ :=
@@ -265,7 +269,6 @@ Section authenticatable.
     match t with
     | tprod t1 t2 => prod_is_ser' v s (s_is_ser_deser t1) (s_is_ser_deser t2)
     | tsum t1 t2 => sum_is_ser' v s (s_is_ser_deser t1) (s_is_ser_deser t2)
-    | toption t1 => option_is_ser' v s (s_is_ser_deser t1)
     | tstring => string_is_ser v s
     | tint => int_is_ser v s
     | tauth => ∃ v1, ⌜v = SOMEV v1⌝ ∗ (auth_is_ser_1 v1 s ∨ auth_is_ser_3 v1 s)
@@ -275,7 +278,6 @@ Section authenticatable.
     match t with
     | tprod t1 t2 => prod_is_ser' v s (s_is_ser'' t1) (s_is_ser'' t2)
     | tsum t1 t2 => sum_is_ser' v s (s_is_ser'' t1) (s_is_ser'' t2)
-    | toption t1 => option_is_ser' v s (s_is_ser'' t1)
     | tstring => string_is_ser v s
     | tint => int_is_ser v s
     | tauth => ∃ v1, ⌜v = SOMEV v1⌝ ∗ (auth_is_ser_1 v1 s ∨ auth_is_ser_2 v1 s)
@@ -285,15 +287,253 @@ Section authenticatable.
     match t with
     | tprod t1 t2 => prod_valid_val' v (s_valid_val t1) (s_valid_val t2)
     | tsum t1 t2 => sum_valid_val' v (s_valid_val t1) (s_valid_val t2)
-    | toption t1 => option_valid_val' v (s_valid_val t1)
     | tstring => string_valid_val v
     | tint => int_valid_val v
     | tauth => auth_valid_val v
     end.
 
-  #[global] Instance s_is_ser''_persistent t v s: Persistent (s_is_ser'' t v s).
-  Proof. Admitted.
-  
+  Fixpoint s_deser_valid_val (t : evi_type) (v : val) : iProp Σ :=
+    match t with
+    | tprod t1 t2 => prod_valid_val' v (s_deser_valid_val t1) (s_deser_valid_val t2)
+    | tsum t1 t2 => sum_valid_val' v (s_deser_valid_val t1) (s_deser_valid_val t2)
+    | tstring => string_valid_val v
+    | tint => int_valid_val v
+    | tauth => auth_deser_valid_val v
+    end.
+
+  #[global] Instance s_valid_val_persistent t v: Persistent (s_valid_val t v).
+  Proof. revert v; induction t => v; simpl; apply _. Qed.
+
+  Fixpoint val_eq (t : evi_type) (v1 v2 : val) : iProp Σ :=
+    match t with
+    | tprod t1 t2 =>
+        ∃ v11 v12 v21 v22,
+          ⌜v1 = (v11, v12)%V ∧ v2 = (v21, v22)%V⌝ ∗ val_eq t1 v11 v21 ∗ val_eq t2 v12 v22
+    | tsum t1 t2 => 
+        ∃ v1' v2',
+          (⌜v1 = InjLV v1' ∧ v2 = InjLV v2'⌝ ∗ val_eq t1 v1' v2') ∨
+            (⌜v1 = InjRV v1' ∧ v2 = InjRV v2'⌝ ∗ val_eq t2 v1' v2')
+    | tstring => ∃ (s: string), ⌜v1 = #s ∧ v2 = #s⌝
+    | tint => ∃ (i: nat), ⌜v1 = #i ∧ v2 = #i⌝
+    | tauth =>
+        ⌜v1 = NONEV ∧ v2 = NONEV⌝ ∨
+          (∃ (h: string), (⌜v1 = SOMEV (InjLV #h)⌝ ∨
+                   (∃ (susp : loc), ⌜v1 = SOMEV (InjRV #susp)⌝ ∗ susp ↦□ InjRV #h)) ∧
+                  (⌜v2 = SOMEV (InjLV #h)⌝ ∨
+                     (∃ (susp : loc), ⌜v2 = SOMEV (InjRV #susp)⌝ ∗ susp ↦□ InjRV #h)))
+    end.
+        
+  Lemma evi_type_ser''_inj (t1 t2 : evi_type) v1 v2 s :
+    (s_is_ser'' t1 v1 s ∨ s_is_ser_deser t1 v1 s) -∗ s_is_ser'' t2 v2 s -∗ val_eq t1 v1 v2.
+  Proof. 
+    iInduction t1 as [| | | |] forall (t2 v1 v2 s).
+    - iIntros "Ht1 Ht2".
+      iDestruct "Ht1" as "[Ht1|Ht1]".
+      + iDestruct "Ht1" as (?????) "(Ht11 & Ht12)".
+        destruct H as [-> ->].
+        destruct t2 => /=; simplify_eq.
+        * iDestruct "Ht2" as (?????) "(Ht21 & Ht22)".
+          destruct H as [-> H]. simplify_eq.
+          iExists _, _, _, _. iSplit; [eauto|].
+          iPoseProof ("IHt1_2" with "[Ht12] Ht22") as "Ht32".
+          { by iLeft. }
+          iPoseProof ("IHt1_1" with "[Ht11] Ht21") as "Ht31".
+          { by iLeft. }
+          iFrame.
+        * iDestruct "Ht2" as (??) "[(Ht2&%)|(Ht2&%)]";
+            destruct H; simplify_eq.
+          { exfalso. by eapply prod_ser_inl_ser_neq. }
+          { exfalso. by eapply prod_ser_inr_ser_neq. }
+        * iDestruct "Ht2" as (?) "(%&%)".
+          iExFalso. by eapply prod_ser_string_ser_neq in H0.
+        * iDestruct "Ht2" as (?) "(%&%)".
+          iExFalso. by eapply prod_ser_int_ser_neq in H0.
+        * admit.
+      + iDestruct "Ht1" as (?????) "(Ht11 & Ht12)".
+        destruct H as [-> ->].
+        destruct t2 => /=; simplify_eq.
+        * iDestruct "Ht2" as (?????) "(Ht21 & Ht22)".
+          destruct H as [-> H]. simplify_eq.
+          iExists _, _, _, _. iSplit; [eauto|].
+          iPoseProof ("IHt1_2" with "[Ht12] Ht22") as "Ht32".
+          { by iRight. }
+          iPoseProof ("IHt1_1" with "[Ht11] Ht21") as "Ht31".
+          { by iRight. }
+          iFrame.
+        * iDestruct "Ht2" as (??) "[(Ht2&%)|(Ht2&%)]";
+            destruct H; simplify_eq.
+          { exfalso. by eapply prod_ser_inl_ser_neq. }
+          { exfalso. by eapply prod_ser_inr_ser_neq. }
+        * iDestruct "Ht2" as (?) "(%&%)".
+          iExFalso. by eapply prod_ser_string_ser_neq in H0.
+        * iDestruct "Ht2" as (?) "(%&%)".
+          iExFalso. by eapply prod_ser_int_ser_neq in H0.
+        * admit.
+    - admit.
+    - admit.
+    - admit.
+    - iIntros "Ht1 Ht2".
+      iDestruct "Ht1" as "[Ht1|Ht1]".
+      + iDestruct "Ht1" as (?->) "[Ht1|Ht1]".
+        * iDestruct "Ht1" as (?) "(-> & Ht1)".
+          destruct t2 => /=; simplify_eq.
+          -- iDestruct "Ht1" as "[(% & ->)|(% & % & (% & %) & Hser)]"; [done|].
+             simplify_eq.
+             iDestruct "Ht2" as (?????) "(Ht21 & Ht22)".
+             destruct H as [-> H].
+             simplify_eq.
+             exfalso. by eapply prod_ser_some_ser_neq.
+          -- iDestruct "Ht1" as "[(% & ->)|(% & % & (% & %) & Hser)]"; [done|].
+             simplify_eq.
+             iDestruct "Ht2" as (??) "[(Ht2&%)|(Ht2&%)]";
+               destruct H; simplify_eq.
+          -- iDestruct "Ht1" as "[(% & ->)|(% & % & (% & %) & (% & -> & ->))]"; [done|].
+             simplify_eq.
+             iDestruct "Ht2" as (?) "(%&%)". simplify_eq.
+          -- iDestruct "Ht1" as "[(% & ->)|(% & % & (% & %) & (% & -> & ->))]"; [done|].
+             simplify_eq.
+             iDestruct "Ht2" as (?) "(%&%)". simplify_eq.
+          -- iDestruct "Ht1" as "[(% & ->)|(% & % & (% & %) & (% & -> & ->))]"; [done|].
+             simplify_eq.
+             iDestruct "Ht2" as (?->) "[(% & -> & Ht2)|(% & % & -> & #Hloc & Ht2)]"; iFrame.
+             { iDestruct "Ht2" as "[(% & %)|(% & % & (% & %) & (% & -> & ->))]"; [done|].
+               simplify_eq. iRight. iExists _. iSplit; iLeft; eauto. }            
+             iRight. iExists _. iSplit.
+             { iLeft. eauto. }
+             iDestruct "Ht2" as "[(% & %)|(% & % & (% & %) & (% & % & %))]"; simplify_eq.
+             iRight. iExists _. eauto.
+        * iDestruct "Ht1" as (??->) "(Hloc & Ht1)".
+          destruct t2 => /=; simplify_eq.
+          -- iDestruct "Ht1" as "[(% & ->)|(% & % & (% & %) & Hser)]"; [done|].
+             simplify_eq.
+             iDestruct "Ht2" as (?????) "(Ht21 & Ht22)".
+             destruct H as [-> H].
+             simplify_eq.
+             exfalso. by eapply prod_ser_some_ser_neq.
+          -- iDestruct "Ht1" as "[(% & ->)|(% & % & (% & %) & Hser)]"; [done|].
+             simplify_eq.
+             iDestruct "Ht2" as (??) "[(Ht2&%)|(Ht2&%)]";
+               destruct H; simplify_eq.
+          -- iDestruct "Ht1" as "[(% & ->)|(% & % & (% & %) & (% & -> & ->))]"; [done|].
+             simplify_eq.
+             iDestruct "Ht2" as (?) "(%&%)". simplify_eq.
+          -- iDestruct "Ht1" as "[(% & ->)|(% & % & (% & %) & (% & -> & ->))]"; [done|].
+             simplify_eq.
+             iDestruct "Ht2" as (?) "(%&%)". simplify_eq.
+          -- iDestruct "Ht1" as "[(% & ->)|(% & % & (% & %) & (% & -> & ->))]"; [done|].
+             simplify_eq.
+             iDestruct "Ht2" as (?->) "[(% & -> & Ht2)|(% & % & -> & #Hloc1 & Ht2)]"; iFrame.
+             { iDestruct "Ht2" as "[(% & %)|(% & % & (% & %) & (% & -> & ->))]"; [done|].
+               simplify_eq. iRight. iExists _. iSplit; [iRight|iLeft]; eauto. }
+             iRight. iExists _. iSplit.
+             { iRight. eauto. }
+             iDestruct "Ht2" as "[(% & %)|(% & % & (% & %) & (% & % & %))]"; simplify_eq.
+             iRight. iExists _. eauto.
+      + iDestruct "Ht1" as (?->) "[Ht1|Ht1]".
+        * iDestruct "Ht1" as (?) "(-> & Ht1)".
+          destruct t2 => /=; simplify_eq.
+          -- iDestruct "Ht1" as "[(% & ->)|(% & % & (% & %) & Hser)]"; [done|].
+             simplify_eq.
+             iDestruct "Ht2" as (?????) "(Ht21 & Ht22)".
+             destruct H as [-> H].
+             simplify_eq.
+             exfalso. by eapply prod_ser_some_ser_neq.
+          -- iDestruct "Ht1" as "[(% & ->)|(% & % & (% & %) & Hser)]"; [done|].
+             simplify_eq.
+             iDestruct "Ht2" as (??) "[(Ht2&%)|(Ht2&%)]";
+               destruct H; simplify_eq.
+          -- iDestruct "Ht1" as "[(% & ->)|(% & % & (% & %) & (% & -> & ->))]"; [done|].
+             simplify_eq.
+             iDestruct "Ht2" as (?) "(%&%)". simplify_eq.
+          -- iDestruct "Ht1" as "[(% & ->)|(% & % & (% & %) & (% & -> & ->))]"; [done|].
+             simplify_eq.
+             iDestruct "Ht2" as (?) "(%&%)". simplify_eq.
+          -- iDestruct "Ht1" as "[(% & ->)|(% & % & (% & %) & (% & -> & ->))]"; [done|].
+             simplify_eq.
+             iDestruct "Ht2" as (?->) "[(% & -> & Ht2)|(% & % & -> & #Hloc & Ht2)]"; iFrame.
+             { iDestruct "Ht2" as "[(% & %)|(% & % & (% & %) & (% & -> & ->))]"; [done|].
+               simplify_eq. iRight. iExists _. iSplit; iLeft; eauto. }            
+             iRight. iExists _. iSplit.
+             { iLeft. eauto. }
+             iDestruct "Ht2" as "[(% & %)|(% & % & (% & %) & (% & % & %))]"; simplify_eq.
+             iRight. iExists _. eauto.
+        * iDestruct "Ht1" as (??->) "(Hloc & Ht1)".
+          destruct t2 => /=; simplify_eq.
+          -- iDestruct "Ht1" as "[(% & ->)|(% & % & (% & %) & Hser)]"; [|done].
+             simplify_eq.
+             iDestruct "Ht2" as (?????) "(Ht21 & Ht22)".
+             destruct H as [-> H].
+             exfalso. by eapply prod_ser_none_ser_neq.
+          -- iDestruct "Ht1" as "[(% & ->)|(% & % & (% & %) & Hser)]"; [|done].
+             simplify_eq.
+             iDestruct "Ht2" as (??) "[(Ht2&%)|(Ht2&%)]";
+               destruct H; simplify_eq.
+          -- iDestruct "Ht1" as "[(% & ->)|(% & % & (% & %) & (% & -> & ->))]"; [|done].
+             simplify_eq.
+             iDestruct "Ht2" as (?) "(%&%)". simplify_eq.
+          -- iDestruct "Ht1" as "[(% & ->)|(% & % & (% & %) & (% & -> & ->))]"; [|done].
+             simplify_eq.
+             iDestruct "Ht2" as (?) "(%&%)". simplify_eq.
+          -- iDestruct "Ht1" as "[(% & ->)|(% & % & (% & %) & (% & -> & ->))]"; [|done].
+             simplify_eq.
+             iDestruct "Ht2" as (?->) "[(% & -> & Ht2)|(% & % & -> & #Hloc1 & Ht2)]"; iFrame;
+               iDestruct "Ht2" as "[(% & %)|(% & % & (% & %) & (% & -> & ->))]"; done.
+  Admitted.
+
+  Lemma deser_valid :
+    ∀ t v s, s_is_ser_deser t v s -∗ s_deser_valid_val t v.
+  Proof.
+    iIntros (???) "Hser".
+    iInduction t as [| | | |] forall (v s); iSimpl; iSimpl in "Hser".
+    - iDestruct "Hser" as (????) "((-> & ->) & H1 & H2)".
+      iPoseProof ("IHt1" with "H1") as "H1".
+      iPoseProof ("IHt2" with "H2") as "H2".
+      iExists v1, v2.
+      iSplit; [done|iFrame].
+    - iDestruct "Hser" as (??) "[(H & %)|(H & %)]".
+      + destruct H as [-> _]. iExists _. iLeft. iSplit; [done|].
+        iApply ("IHt1" with "H").
+      + destruct H as [-> _]. iExists _. iRight. iSplit; [done|].
+        iApply ("IHt2" with "H").
+    - iDestruct "Hser" as "%Hser". destruct Hser as (? & -> & _). iExists _. done.
+    - iDestruct "Hser" as "%Hser". destruct Hser as (? & -> & _). iExists _. done.
+    - iDestruct "Hser" as (? ->) "[(% & -> & Hser)|(% & % & -> & Hsusp & Hser)]".
+      + iExists _. iSplit; [done|].
+        iLeft. eauto.
+      + iExists _.
+        iSplit; [done|].
+        iRight. iExists _. iSplit; [done|]. iExists _. iFrame.
+  Qed.            
+
+  Lemma deser_valid_weak E :
+    ∀ t v, s_deser_valid_val t v ⊢ |={E}=> s_valid_val t v.
+  Proof.
+    iIntros (??) "Hdvalid".
+    iInduction t as [| | | |] forall (v); iSimpl; iSimpl in "Hdvalid".
+    - iDestruct "Hdvalid" as (??->) "[H1 H2]".
+      iPoseProof ("IHt1" with "H1") as "H1".
+      iPoseProof ("IHt2" with "H2") as "H2".
+      iExists v1, v2.
+      iMod "H1". iMod "H2".
+      iModIntro. iSplit; [done|iFrame].
+    - iDestruct "Hdvalid" as (?) "[[-> H]|[-> H]]".
+      + iPoseProof ("IHt1" with "H") as "H". iMod "H".
+        iModIntro. iExists _. iLeft. iSplit; [done|iExact "H"].
+      + iPoseProof ("IHt2" with "H") as "H". iMod "H".
+        iModIntro. iExists _. iRight. iSplit; [done|iExact "H"].
+    - by iModIntro.
+    - by iModIntro.
+    - iDestruct "Hdvalid" as (? ->) "[(% & ->)|(% & -> & % & Hsusp)]".
+      + iExists _. iModIntro. iSplit; [done|].
+        iLeft. eauto.
+      + iExists _.
+        iMod (na_inv_alloc seqG_name E (authValidN #susp) (valid_auth_inv susp) with "[Hsusp]") as "Hinv".
+        { iNext. iRight. eauto. }
+        iModIntro.
+        iSplit; [done|].
+        iRight. eauto.
+  Qed.
+        
   #[global] Instance : Inhabited evi_type.
   Proof. constructor. apply tstring. Qed.
 
@@ -310,39 +550,79 @@ Section authenticatable.
     match t with
     | tprod t1 t2 => prod_count (evi_type_count t1) (evi_type_count t2)
     | tsum t1 t2 => sum_count (evi_type_count t1) (evi_type_count t2)
-    | toption t1 => option_count (evi_type_count t1)
     | tstring => string_count
     | tint => int_count
     | tauth => auth_count
     end.
 
+  Definition count_auth_inv (susp: loc) (c: nat) : iProp Σ :=
+     ((∃ (h : string), susp ↦□ (InjRV #h) ∗ ⌜c = 0⌝) ∨
+        (∃ (pid : nat), susp ↦ (InjLV #pid) ∗ ⌜c = 1⌝)).
+
   Fixpoint count_is_correct (t : evi_type) (v : val) (c : nat) : iProp Σ :=
     match t with
     | tprod t1 t2 =>
         ∃ (c1 c2 : nat) (v1 v2 : val),
-          ⌜v = (v1, v2)%V⌝ ∧ count_is_correct t1 v1 c1 ∧ count_is_correct t2 v2 c2 ∧ ⌜(c1 + c2)%nat = c⌝
+          ⌜v = (v1, v2)%V⌝ ∗ count_is_correct t1 v1 c1 ∗ count_is_correct t2 v2 c2 ∗ ⌜(c1 + c2)%nat = c⌝
     | tsum t1 t2 =>
-        (∃ (v1 : val), ⌜v = InjLV v1⌝ ∧ count_is_correct t1 v1 c) ∨
-          (∃ (v2 : val), ⌜v = InjRV v2⌝ ∧ count_is_correct t2 v2 c)
-    | toption t1 =>
-        ⌜(v = NONEV ∧ c = 0)⌝ ∨ (∃ (v1 : val), ⌜v = SOMEV v1⌝ ∧ count_is_correct t1 v1 c)
-    | tstring | tint => ⌜c = 0⌝
+        (∃ (v1 : val), ⌜v = InjLV v1⌝ ∗ count_is_correct t1 v1 c) ∨
+          (∃ (v2 : val), ⌜v = InjRV v2⌝ ∗ count_is_correct t2 v2 c)
+    | tstring => string_valid_val v ∧ ⌜c = 0⌝
+    | tint => int_valid_val v ∧ ⌜c = 0⌝
     | tauth =>
-        (⌜v = NONEV ∧ c = 0⌝) ∨
-          (∃ v1,
-              ⌜v = SOMEV v1⌝ ∧
-                (∃ (l : val), ⌜v1 = InjLV l ∧ c = 0⌝) ∨ 
-                (∃ (susp : loc),
-                    ⌜v1 = InjRV #susp⌝ ∧
-                      ((∃ (h : string), susp ↦{DfracDiscarded} (InjRV #h) ∧ ⌜c = 0⌝) ∨
-                         (∃ (pid: nat), susp ↦ (InjLV #pid) ∧ ⌜c = 1⌝))))
-    end.
+        (∃ v1, ⌜v = SOMEV v1⌝ ∧
+                 ((∃ (h : string), ⌜v1 = InjLV #h ∧ c = 0⌝) ∨ 
+                    (∃ (susp : loc),
+                        ⌜v1 = InjRV #susp⌝ ∗ seq_inv (authCountN #susp) (count_auth_inv susp c))))
+  end.
+
+  #[global] Instance count_is_correct_persistent t v c: Persistent (count_is_correct t v c).
+  Proof. revert v c; induction t => v c; simpl; apply _. Qed.
+
+(*  Lemma count_valid t v :
+    ∀ E1 c, ∃ E2, seq_tok E1 ∗ count_is_correct t v c  ={E1,E2}=∗ seq_tok E2 ∗ s_valid_val t v.
+  Proof.
+    iIntros (?). eexists _. iIntros "(Htok & Hcount)".
+    iInduction t as [| | | |] forall (E1 v c); iSimpl; iSimpl in "Hcount".
+    - iDestruct "Hcount" as (???? -> ) "(Hcount1 & Hcount2 & %)". simplify_eq.
+      iPoseProof ("IHt1" with "Htok Hcount1") as "H1".
+      iMod "H1" as "(Htok & H1)".
+      iPoseProof ("IHt2" with "Htok Hcount2") as "H2".
+      iMod "H2" as "(Htok & H2)". iFrame.
+      iModIntro. iFrame. eauto.
+    - iDestruct "Hcount" as "[(%&->&Hcount)|(%&->&Hcount)]".
+      + iPoseProof ("IHt1" with "Htok Hcount") as "H".
+        iMod "H" as "(Htok & H)". iFrame.
+        iModIntro. iExists _. iLeft. eauto.
+      + iPoseProof ("IHt2" with "Htok Hcount") as "H".
+        iMod "H" as "(Htok & H)". iFrame.
+        iModIntro. iExists _. iRight. eauto.
+    - iFrame. by iDestruct "Hcount" as "(H&%)".
+    - iFrame. by iDestruct "Hcount" as "(H&%)".
+    - iFrame. iDestruct "Hcount" as (??) "[(%&->&->)|(%&->&Hsusp)]".
+      + iModIntro. iExists _. iSplit; [done|]. eauto.
+      + iExists _.
+        iMod (na_inv_acc with "Hsusp") as "Hinv". *)
+        
                                                  
-  Definition ser_spec (ser : val) (t : evi_type) (A : lrel Σ) : iProp Σ :=
-    ∀ (v1 v2 : val),
-      {{{ ▷ A v1 v2 }}}
+  Definition ser_spec_3 (ser : val) (t : evi_type) : iProp Σ :=
+    ∀ (v1 : val) (c: nat),
+      {{{ ▷ (count_is_correct t v1 c ∗ seq_tok ⊤) }}}
         ser v1
-      {{{ o, RET $o; if o is Some s then s_is_ser'' t v1 s else True }}}.
+        {{{ o, RET $o; seq_tok ⊤ ∗ if o is Some s then s_is_ser'' t v1 s else True }}}.
+        
+                                                 
+  Definition ser_spec_2 (ser : val) (t : evi_type) : iProp Σ :=
+    ∀ (v1 : val),
+      {{{ ▷ (s_valid_val t v1 ∗ seq_tok ⊤) }}}
+        ser v1
+        {{{ o, RET $o; seq_tok ⊤ ∗ if o is Some s then s_is_ser'' t v1 s else True }}}.
+
+  Definition ser_spec (A : lrel Σ) (ser : val) (t : evi_type) : iProp Σ :=
+    ∀ (v1 v2 : val),
+      {{{ ▷ (A v1 v2 ∗ seq_tok ⊤) }}}
+        ser v1
+      {{{ o, RET $o; seq_tok ⊤ ∗ if o is Some s then s_is_ser'' t v1 s else True }}}.
 
   Definition deser_spec (deser : val) (t : evi_type) : iProp Σ :=
     ∀ (pid : nat),
@@ -363,98 +643,114 @@ Section authenticatable.
 
   Definition count_spec (count : val) (t : evi_type): iProp Σ :=
     ∀ (v1 : val),
-      {{{ ▷ s_valid_val t v1 }}}
+      {{{ ▷ s_deser_valid_val t v1 }}}
         count v1
       {{{ v, RET v; ∃ (c : nat), ⌜v = #c⌝ ∧ count_is_correct t v1 c }}}.
 
   Definition lrel_evidence' (A : lrel Σ) : lrel Σ :=
     LRel (λ v1 v2,
         ∃ (t : evi_type) (ser deser count : val),
-          ⌜v1 = (ser, deser, count)%V⌝ ∗ ser_spec ser t A ∗ count_spec count t ∗
+          ⌜v1 = (ser, deser, count)%V⌝ ∗ ser_spec A ser t ∗ ser_spec_2 ser t ∗ ser_spec_3 ser t ∗ count_spec count t ∗
             deser_spec deser t)%I.
 
   Program Definition lrel_evidence : kindO Σ (⋆ ⇒ ⋆)%kind := λne A, lrel_evidence' A.
   Next Obligation.
     intros ??????.
-    rewrite /lrel_car/= /ser_spec /count_spec.
+    rewrite /lrel_car/= /ser_spec /count_spec /deser_spec.
     solve_proper.
   Qed.
 
   Lemma prod_ser'_spec_ser (HA HB : val → iProp Σ) (tA tB : evi_type) (serA serB v vA vB : val) :
     (▷ ⌜v = (vA, vB)%V⌝) -∗
-    ({{{ ▷ HA vA }}}
+    ({{{ ▷ (HA vA ∗ seq_tok ⊤) }}}
         serA vA
-      {{{ o, RET $o; if o is Some s then s_is_ser'' tA vA s else True }}}) -∗
-    ({{{ ▷ HB vB }}}
+      {{{ o, RET $o; seq_tok ⊤ ∗ if o is Some s then s_is_ser'' tA vA s else True }}}) -∗
+    ({{{ ▷ (HB vB ∗ seq_tok ⊤) }}}
         serB vB
-      {{{ o, RET $o; if o is Some s then s_is_ser'' tB vB s else True }}}) -∗
-    {{{ ▷ prod_valid_val' v HA HB }}}
+      {{{ o, RET $o; seq_tok ⊤ ∗ if o is Some s then s_is_ser'' tB vB s else True }}}) -∗
+    {{{ ▷ (prod_valid_val' v HA HB ∗ seq_tok ⊤) }}}
       prod_ser''' serA serB v
-      {{{ o, RET $o; if o is Some s then prod_is_ser' v s (s_is_ser'' tA) (s_is_ser'' tB) else True }}}.
+      {{{ o, RET $o; seq_tok ⊤ ∗ if o is Some s then prod_is_ser' v s (s_is_ser'' tA) (s_is_ser'' tB) else True }}}.
   Proof.
-    iIntros "#Hv #HA #HB % !# Hp HΦ".
+    iIntros "#Hv #HA #HB % !# (Hp & Htok) HΦ".
     rewrite /prod_ser''' /prod_is_ser.
     wp_pures.
     iDestruct "Hp" as (???) "[H1 H2]". iSimplifyEq.
     wp_pures.
-    wp_apply ("HA" with "H1").
-    iIntros (o) "#Ho". destruct o; last first.
-    { wp_pures. by iApply ("HΦ" $! None). }
+    wp_apply ("HA" with "[$H1 $Htok]").
+    iIntros ([]); last first.
+    { iIntros "(Htok & _)". wp_pures. iApply ("HΦ" $! None). by iFrame. }
+    iIntros "(Htok & HserA)".
     wp_pures.
-    wp_apply ("HB" with "H2").
-    iIntros (o) "#Ho1". destruct o; last first.
-    { wp_pures. by iApply ("HΦ" $! None). }
+    wp_apply ("HB" with "[$H2 $Htok]").
+    iIntros ([]); last first.
+    { iIntros "(Htok & _)". wp_pures. iApply ("HΦ" $! None). by iFrame. }
+    iIntros "(Htok & HserB)".
     wp_pures.
     iApply ("HΦ" $! (Some _)).
-    iModIntro.
-    iExists vA, vB, s, s0; iSplit; auto.
+    iModIntro. iFrame. eauto.
   Qed.
   
 End authenticatable.
 
-Section proof.
-  Context `{!authG Σ} (N : namespace).
+Instance s_is_ser''_persistent `{heapGS_gen hlc Σ, seqG Σ} t v s: Persistent (s_is_ser'' t v s).
+Proof. revert v s; induction t => v s; simpl; apply _. Qed.
 
-  Definition authSerBaseN : namespace := N .@ "auth_ser".
-  Definition authSerN (v : val) : namespace := N .@ v.
+Section proof.
+  Context `{!authG Σ, !seqG Σ} (N : namespace).
+
+  Definition authSerProofN (v : val) : namespace := N .@ "auth_ser_proof" .@ v.
 
   Lemma refines_Auth_pair Θ (Δ : ctxO Σ Θ) :
     ⊢ ⟦ ∀: ⋆; ⋆, var2 var1 → var2 var0 → var2 (var1 * var0) ⟧
-      (ext Δ lrel_evidence) v_Auth_pair i_Auth_pair.
+      (ext Δ (lrel_evidence N)) v_Auth_pair i_Auth_pair.
   Proof.
     interp_unfold.
     iIntros (A ??) "!# _".
-    iIntros (??) "Hi".
+    iIntros (??) "(Hi & Htok)".
     rewrite /v_Auth_pair /i_Auth_pair.
     i_pures; wp_pures.
     iModIntro. iFrame.
     iIntros (B ??) "!# _".
-    iIntros (??) "Hi".
+    iIntros (??) "(Hi & Htok)".
     i_pures; wp_pures.
     iModIntro. iFrame.
     iIntros (??) "!# HA".
     interp_unfold! in "HA".
-    iDestruct "HA" as (tA serA deserA countA ->) "(#HserA & #HcountA & #HdeserA)". clear.
-    iIntros (??) "Hi".
+    iDestruct "HA" as (tA serA deserA countA ->) "(#HserA & #Hser2A & #Hser3A & #HcountA & #HdeserA)". clear.
+    iIntros (??) "(Hi & Htok)".
     i_pures; wp_pures.
     iModIntro. iFrame.
     iIntros (??) "!# HB".
     interp_unfold! in "HB".
-    iDestruct "HB" as (tB serB deserB countB ->) "(#HserB & #HcountB & #HdeserB)". clear.
-    iIntros (??) "Hi".
+    iDestruct "HB" as (tB serB deserB countB ->) "(#HserB & #Hser2B & #Hser3B & #HcountB & #HdeserB)". clear.
+    iIntros (??) "(Hi & Htok)".
     i_pures; wp_pures. clear.
     rewrite /prod_scheme /prod_ser'' /prod_deser /prod_count.
     wp_pures. iFrame. iModIntro.
     interp_unfold!.
     iExists (tprod tA tB), _, _, _.
-    iSplit; [done|]. clear. iSplit; [|iSplit].
-    - iIntros (v1 v2 ?) "!# Hp H".
+    iSplit; [done|]. clear. iSplit; [|iSplit; [|iSplit; [|iSplit]]].
+    - iIntros (v1 v2 ?) "!# (Hp & Htok) H".
       iDestruct "Hp" as (w1 w2 u1 u2) "(>-> & >-> & #HA & #HB)".
       iSimpl in "H".
-      wp_apply (prod_ser'_spec_ser (λ v1, A v1 w2)%I (λ v1, B v1 u2)%I) => /=; [done| | | |done].  
-      { iIntros (?) "!# _ H". by wp_apply ("HserA" with "HA"). }
-      { iIntros (?) "!# _ H". by wp_apply ("HserB" with "HB"). }
+      wp_apply (prod_ser'_spec_ser (λ v1, A v1 w2) (λ v1, B v1 u2) with "[] [] [] [$Htok]") => /=; [done| | | |done].  
+      { iIntros (?) "!# Hp H". by wp_apply ("HserA" with "Hp"). }
+      { iIntros (?) "!# Hp H". by wp_apply ("HserB" with "Hp"). }
       iExists _, _. eauto.
+    - iIntros (v1 ?) "!# (Hp & Htok) H". iSimpl in "Hp".
+      iDestruct "Hp" as (w1 w2) "(>-> & HA & HB)".
+      wp_apply (prod_ser'_spec_ser (s_valid_val _ tA) (s_valid_val _ tB) with "[] [] [] [HA HB $Htok]") => /=; [done| | | |done].  
+      { iIntros (?) "!# Hp H". by wp_apply ("Hser2A" with "Hp"). }
+      { iIntros (?) "!# Hp H". by wp_apply ("Hser2B" with "Hp"). }
+      iNext. iFrame. eauto.
+    - iIntros (v1 c ?) "!# (Hc & Htok) H".
+      iDestruct "Hc" as (????) "(>-> & HA & HB & >%)".
+      iSimpl in "H".
+      wp_apply (prod_ser'_spec_ser (λ v1, count_is_correct _ tA v1 c1) (λ v2, count_is_correct _ tB v2 c2) with "[] [] [] [HA HB $Htok]") => /=; [done| | | |done].
+      { iIntros (?) "!# Hc H". by wp_apply ("Hser3A" with "Hc"). }
+      { iIntros (?) "!# Hc H". by wp_apply ("Hser3B" with "Hc"). }
+      iNext. iFrame. eauto.
     - iIntros (??) "!# Hp HΨ". wp_pures.
       iDestruct "Hp" as (?? ->) "(HA & HB)".
       wp_pures. rewrite /count_spec.
@@ -469,53 +765,59 @@ Section proof.
       iExists (c0+c). iSplit; [iPureIntro; f_equal|].
       { by rewrite Nat2Z.inj_add. }
       iExists _, _, _, _.
-      iSplit; eauto.
+      iSplit; iFrame; done.
     - iIntros (pid ?) "!# _ HΨ".
       wp_pures.
       wp_apply "HdeserB"; [done|]. iIntros "%deparB #HdeparB".
       wp_apply "HdeserA"; [done|]. iIntros "%deparA #HdeparA".
       wp_pures. iModIntro. iApply "HΨ".
       iIntros (s ?) "!# _ HΨ".
-      wp_apply prod_deser'_sound; done.       
+      wp_apply prod_deser'_sound; auto.
   Qed.
   
   Lemma refines_Auth_sum Θ (Δ : ctxO Σ Θ) :
     ⊢ ⟦ ∀: ⋆; ⋆, var2 var1 → var2 var0 → var2 (var1 + var0) ⟧
-      (ext Δ lrel_evidence) v_Auth_sum i_Auth_sum.
+      (ext Δ (lrel_evidence N)) v_Auth_sum i_Auth_sum.
   Proof. Admitted.
 
   Lemma refines_Auth_string :
-    ⊢ lrel_evidence lrel_string v_Auth_string i_Auth_string.
+    ⊢ (lrel_evidence N) lrel_string v_Auth_string i_Auth_string.
   Proof. Admitted.
 
   Lemma refines_Auth_int :
-    ⊢ lrel_evidence lrel_int v_Auth_int i_Auth_int.
+    ⊢ (lrel_evidence N) lrel_int v_Auth_int i_Auth_int.
   Proof. Admitted.
 
   Lemma refines_Auth_mu Θ (Δ : ctxO Σ Θ) :
     ⊢ ⟦ ∀: ⋆ ⇒ ⋆, var1 (var0 (μ: ⋆; var1 var0)) → var1 (μ: ⋆; var1 var0) ⟧
-      (ext Δ lrel_evidence) v_Auth_mu i_Auth_mu.
+      (ext Δ (lrel_evidence N)) v_Auth_mu i_Auth_mu.
   Proof.
     rewrite /lrel_car/=.
-    iIntros (A v1 v2) "!# _". iIntros (??) "Hi".
+    iIntros (A v1 v2) "!# _". iIntros (??) "(Hi & Htok)".
     rewrite /i_Auth_mu /v_Auth_mu.
     i_pures. wp_pures.
     iFrame. iModIntro. clear.
     interp_unfold!.
     iIntros (??) "!# H".
-    iIntros (??) "Hi".
+    iIntros (??) "(Hi & Htok)".
     interp_unfold! in "H".
-    iDestruct "H" as "(%t & %ser & %deser & %count & -> & #Hser & #Hcount & #Hdeser)".
+    iDestruct "H" as "(%t & %ser & %deser & %count & -> & #Hser & #Hser2 & #Hser3 & #Hcount & #Hdeser)".
     i_pures. wp_pures.
     iFrame. iModIntro.
     interp_unfold!.
     iExists t, _, _, _. iSplit; [done|].
-    clear. iSplit; [|iSplit].
-    - iIntros (v1 v2 Ψ) "!# Hs HΨ".
+    clear. iSplit; [|iSplit]; [| |iSplit; [|iSplit]].
+    - iIntros (v1 v2 Ψ) "!# (#Hs & Htok) HΨ".
       wp_pures.
       rewrite interp_rec_star_unfold.
       rewrite interp_unseal /=.
-      by wp_apply ("Hser" with "Hs").
+      wp_apply ("Hser" with "[Htok]"); [by iFrame|done].
+    - iIntros (v1 Ψ) "!# (Hs & Htok) HΨ".
+      wp_pures.
+      wp_apply ("Hser2" with "[Hs Htok]"); [by iFrame|done].
+    - iIntros (v1 c Ψ) "!# (Hs & Htok) HΨ".
+      wp_pures.
+      wp_apply ("Hser3" with "[Hs Htok]"); [by iFrame|done].
     - iIntros (??) "!# Hp HΨ". wp_pures.
       by iApply ("Hcount" with "Hp").
     - iIntros (pid Ψ) "!# _ HΨ". wp_pures.
@@ -523,26 +825,39 @@ Section proof.
       iIntros (s ?) "!# _ HΨ". wp_pures.
       wp_apply "Hdeser"; [done|].
       iIntros (depar) "HΨ1".
-      by iApply "HΨ1".
+      iApply "HΨ1"; [done|].
+      iModIntro.
+      iIntros ([]) "H"; last first.
+      { by iApply "HΨ". }
+      by iApply "HΨ".
   Qed.
 
+  Definition auth_inv (susp : loc) :=
+    ((∃ (s1 : string), hashed s1 ∗ susp ↦□ InjRV #(hash s1)) ∨
+       ∃ (pid : nat), susp ↦ (InjLV #pid))%I.
+
+  Definition auth_some (A : lrel Σ) (v1 v2 : val) : iProp Σ :=
+    (∃ (a1 : val) (t : evi_type) (s1 : string),
+        s_is_ser'' t a1 s1 ∗ A a1 v2 ∗
+          ((hashed s1 ∗ ⌜v1 = InjLV #(hash s1)⌝) ∨
+             (∃ (susp : loc),
+                 ⌜v1 = InjRV #susp⌝ ∗ seq_inv (authSerProofN #susp) (auth_inv susp)))).
+
+  #[global] Instance auth_some_persistent A v1 v2 : Persistent (auth_some A v1 v2).
+  Proof. unfold auth_some. apply _. Qed.
+  
   Definition lrel_auth_some (A : lrel Σ) : lrel Σ :=
-    LRel (λ v1 v2,
-        (∃ (a1 : val) (t : evi_type) (s1 : string),
-            s_is_ser'' t a1 s1 ∗ A a1 v2 ∗ hashed s1 ∗
-              ⌜v1 = InjLV #(hash s1)⌝) ∨
-          (∃ (susp : loc),
-              ⌜v1 = InjRV #susp⌝ ∗
-                inv (authSerN #susp) ((∃ (a1 : val) (t : evi_type) (s1 : string),
-                    s_is_ser'' t a1 s1 ∗ A a1 v2 ∗ hashed s1 ∗
-                      susp ↦{DfracDiscarded} (InjRV #s1)) ∨
-                   (∃ (pid : nat), susp ↦ (InjLV #pid)))))%I.
+    LRel (λ v1 v2, auth_some A v1 v2)%I.
 
   Definition lrel_auth' (A : lrel Σ) : lrel Σ :=
     LRel (λ a1 v2, (∃ v1, ⌜a1 = SOMEV v1⌝ ∗ lrel_auth_some A v1 v2) ∨ ⌜a1 = NONEV⌝)%I.
   
   Program Definition lrel_auth : kindO Σ (⋆ ⇒ ⋆)%kind := λne A, lrel_auth' A.
-  Next Obligation. Admitted.
+  Next Obligation.
+    intros ??????.
+    rewrite /lrel_car/= /lrel_auth' /lrel_auth_some /auth_some.
+  Admitted.
+  
 
   Definition is_proof (v : val) : iProp Σ :=
     ∃ (l : list string), ⌜is_list l v⌝.
@@ -551,88 +866,156 @@ Section proof.
     LRel (λ v1 _, is_proof v1 )%I.
 
   Definition auth_ctx {Θ} (Δ : ctxO Σ Θ) (R : kindO Σ (⋆ ⇒ ⋆)) :=
-    ext (ext (ext Δ lrel_auth) R) lrel_evidence.
+    ext (ext (ext Δ lrel_auth) R) (lrel_evidence N).
 
   Lemma refines_Auth_auth Θ (Δ : ctxO Σ Θ) R :
     ⊢ ⟦ ∀: ⋆, var1 (var3 var0) ⟧
       (auth_ctx Δ R) v_Auth_auth i_Auth_auth.
   Proof.
     iIntros (A ??) "!# _"; rewrite -!/interp.
-    iIntros (??) "Hi".
+    iIntros (??) "(Hi & Htok)".
     rewrite /v_Auth_auth /i_Auth_auth.
     i_pures; wp_pures.
     iModIntro. iFrame.
     rewrite /auth_ctx.
     interp_unfold!.
     iExists tauth, _, _, _.
-    iSplit; [done|]. clear. iSplit; [|iSplit].
-    - iIntros (???) "!# #Hauth H".
+    iSplit; [done|]. clear. iSplit; [|iSplit]; [| |iSplit; [|iSplit]].
+    - iIntros (???) "!# (#Hauth & Htok) H".
       rewrite /auth_ser_v. wp_pure.
       iDestruct "Hauth" as "[(% & -> & Hauth)|->]"; wp_pures; last first.
-      { by iApply ("H" $! None). }
-      iDestruct "Hauth" as "[(%&%&%&Hser&HA&Hhash&%)|(%&%&Hinv)]";
+      { iApply ("H" $! None). by iFrame. }
+      iDestruct "Hauth" as "(%&%&%&Hser&HA&[(Hhash&%)|(%&%&Hinv)])";
         simplify_eq; wp_pures.
       + wp_apply s_ser_spec'.
         { iRight. eauto. }
         iIntros (o) "#Ho". destruct o; last first.
-        { by iApply ("H"  $! None). }
-        iApply ("H" $! (Some _)).
+        { iApply ("H"  $! None). by iFrame. }
+        iApply ("H" $! (Some _)). iFrame.
         iExists _. iSplit; [done|].
         iLeft. iExists _. eauto.
       + wp_bind (!_)%E.
-        iInv "Hinv" as "[(%&%&%&Hser&HA&Hhash&#Hsusp)|(%&Hsusp)]" "Hclose";
-          wp_load.
-        * iMod ("Hclose" with "[Hser HA Hhash Hsusp]") as "_".
-          { iLeft. iFrame "#∗". }
-          iModIntro. wp_pures.
+        iMod (na_inv_acc with "Hinv Htok") as "(Hinv1 & Htok & Hclose)"; [done|done|].
+        iDestruct "Hinv1" as "[(%&#Hhash&#Hsusp)|(%&Hsusp)]".
+        * (* iMod ("Hclose" with "[Htok]") as "Htok".
+          { iFrame. iNext. iLeft. iFrame "∗ #". }
+          wp_pures.
+          iMod ("Hclose" with "[Htok]") as "Htok".
+          { iFrame. iNext. iLeft. iFrame "∗ #". }
           wp_apply s_ser_spec'.
           { iRight. eauto. }
           iIntros (o) "#Ho". destruct o; last first.
           { by iApply ("H" $! None). }
           iApply ("H" $! (Some _)).
+          iFrame.
+          iExists _. iSplit; [done|].
+          iRight. iExists _, _.
+          iSplit; [done|]. iFrame "#". *)
+          wp_load.
+          iDestruct "Hser" as "#Hser".
+          iMod ("Hclose" with "[Hser HA Hhash Hsusp Htok]") as "Htok".
+          { iFrame. iLeft. iFrame "#∗". }
+          wp_pures.
+          wp_apply s_ser_spec'.
+          { iRight. eauto. }
+          iIntros (o) "#Ho". destruct o; last first.
+          { iApply ("H" $! None). iFrame. }
+          iApply ("H" $! (Some _)). iFrame.
+          iExists _. iSplit; [done|].
+          iRight. iExists _, _. eauto.
+        * wp_load.
+          iMod ("Hclose" with "[$Hsusp $Htok]") as "Htok".
+          wp_pures.
+          iApply ("H" $! None). by iFrame.
+    - iIntros (??) "!# (#Hauth & Htok) H".
+      rewrite /auth_ser_v. wp_pure. iSimpl in "Hauth".
+      iDestruct "Hauth" as "(% & -> & [(% & ->)|(%&%&Hinv)])".
+      + wp_pures. wp_apply s_ser_spec'.
+        { iRight. eauto. }
+        iIntros (o) "#Ho". destruct o; last first.
+        { iApply ("H"  $! None). by iFrame. }
+        iApply ("H" $! (Some _)). iFrame.
+        iExists _. iSplit; [done|].
+        iLeft. iExists _. eauto.
+      + simplify_eq. wp_pures. wp_bind (!_)%E.
+        iMod (na_inv_acc with "Hinv Htok") as "([(%&#Hsusp)|(%&Hsusp)] & Htok & Hclose)"; [done|done| |]; wp_load.
+        * iMod ("Hclose" with "[$Htok]") as "Htok".
+          { iLeft. iFrame "#∗". }
+          wp_pures.
+          wp_apply s_ser_spec'.
+          { iRight. eauto. }
+          iIntros (o) "#Ho". destruct o; last first.
+          { iApply ("H" $! None). by iFrame. }
+          iApply ("H" $! (Some _)). iFrame.
           iExists _. iSplit; [done|].
           iRight. iExists _, _.
           eauto.
-        * iMod ("Hclose" with "[Hsusp]") as "_".
+        * iMod ("Hclose" with "[Hsusp $Htok]") as "Htok".
           { iRight. eauto. }
-          iModIntro. wp_pures.
-          by iApply ("H" $! None).
+          wp_pures.
+          iApply ("H" $! None). by iFrame.
+
+    - iIntros (???) "!# (#Hc & Htok) H".
+      rewrite /auth_ser_v. wp_pure. iSimpl in "Hc".
+      iDestruct "Hc" as (?->) "[(% & -> & ->)|(% & -> & Hinv)]".
+      + wp_pures. wp_apply s_ser_spec'.
+        { iRight. eauto. }
+        iIntros (o) "#Ho". destruct o; last first.
+        { iApply ("H"  $! None). by iFrame. }
+        iApply ("H" $! (Some _)). iFrame.
+        iExists _. iSplit; [done|].
+        iLeft. iExists _. eauto.
+      + simplify_eq. wp_pures. wp_bind (!_)%E.
+        iMod (na_inv_acc with "Hinv Htok") as "([(%&#Hsusp&>%)|(%&Hsusp&>%)] & Htok & Hclose)"; [done|done| |]; wp_load.
+        * iMod ("Hclose" with "[$Htok]") as "Htok".
+          { iLeft. by iFrame "#∗". }
+          wp_pures.
+          wp_apply s_ser_spec'.
+          { iRight. eauto. }
+          iIntros (o) "#Ho". destruct o; last first.
+          { iApply ("H" $! None). by iFrame. }
+          iApply ("H" $! (Some _)). iFrame.
+          iExists _. iSplit; [done|].
+          iRight. iExists _, _.
+          eauto.
+        * iMod ("Hclose" with "[Hsusp $Htok]") as "Htok".
+          { iRight. eauto. }
+          wp_pures.
+          iApply ("H" $! None). by iFrame.
+        
     - iIntros (??) "!# Hauth H".
       rewrite /auth_count. wp_pures.
-      iDestruct "Hauth" as "(% & -> & [(% & ->)|Hauth])"; wp_pures.
+      iDestruct "Hauth" as "(% & -> & [(% & ->)|(%&%&%&Hsusp)])"; simplify_eq; wp_pures.
+      { iApply "H". iExists 0. iModIntro. iSplit; [done|].
+        iExists _. eauto. }
+      wp_load. wp_pures.
+      iMod (na_inv_alloc seqG_name ⊤ (authCountN N #susp) (count_auth_inv susp 1) with "[Hsusp]") as "Hinv".
+      { iRight. iExists _. iModIntro. by iFrame. }
+      iApply "H". iExists 1. iModIntro.
+      iSplit; [iPureIntro; f_equal|].
+      iExists _. iSplit; [done|]. iRight. iExists susp. by iFrame.
+      
+      (* iDestruct "Hauth" as "(% & -> & [(% & ->)|(%&%&#Hinv)])"; simplify_eq; wp_pures.
       { iApply "H". iExists 0. iModIntro. iSplit; [done|].
         iRight. iExists _. eauto. }
-      iDestruct "Hauth" as "(% & -> & [(% & Hsusp)|(% & Hsusp)])";
-        simplify_eq; wp_pures.
-      + wp_load. wp_pures.
+      wp_bind (!_)%E.
+      iInv "Hinv" as "[(%&#Hsusp)|(%&Hsusp)]" "Hclose"; wp_load.
+      + iMod ("Hclose" with "[]") as "_".
+        { iLeft. eauto. }
+        iModIntro. wp_pures.
         iApply "H". iExists 0. iModIntro.
         iSplit; [iPureIntro; f_equal|].
-        iRight. iExists _. iRight. iExists _. eauto.
-      + wp_load. wp_pures.
-        iApply "H".
-        iExists 1.
-        iModIntro. iSplit; [iPureIntro; f_equal|].
-        iRight. iExists _. iRight. iExists _. eauto.
+        iRight. iExists _. iRight.
+        iExists _. iSplit; [done|].
+        iLeft. eauto.
+      + iMod ("Hclose" with "[Hsusp]") as "_".
+        { iRight. eauto. }
+        iModIntro. wp_pures.
+        iApply "H". iExists 1. iModIntro.
+        iSplit; [iPureIntro; f_equal|].
+        iRight. iExists _. iRight. iExists susp.
+        iSplit; [done|]. by iRight. *)
         
-        (* iInv "Hinv" as "[(%&%&%&Hser&HA&Hhash&#Hsusp)|(%&Hsusp)]" "Hclose";
-          wp_load.
-        * iMod ("Hclose" with "[Hser HA Hhash Hsusp]") as "_".
-          { iLeft. iFrame "#∗". }
-          iModIntro. wp_pures.
-          iApply "H". iExists 0.
-          iModIntro. iSplit; [done|].
-          iRight.
-          iExists _. iRight. iExists susp.
-          iSplit; [done|]. iLeft.
-          iExists s1. eauto.
-        * iMod ("Hclose" with "[Hsusp]") as "_".
-          { iRight. iFrame "#∗". }
-          iModIntro. wp_pures.
-          iApply "H".
-          
-          iExists 1.
-          iModIntro. iSplit; [iPureIntro; f_equal|].
-          iRight. *)
           
     - iIntros (??) "!# _ H".
       rewrite /auth_deser_v. wp_pures.
@@ -641,12 +1024,20 @@ Section proof.
       wp_pures. wp_apply s_deser_sound; [done|].
       iIntros ([] ?); wp_pures.
       + destruct H as [(->&H)|(?&?&(->&H)&?)]; wp_pures.
-        * wp_alloc susp. wp_pures.
+        * wp_alloc susp as "Hsusp".
+(*          iMod(inv_alloc (authSerN #susp) _ (auth_inv A susp) with "[Hsusp]") as "#Hinv".
+          { iModIntro. iRight. eauto. } *)
+          wp_pures.
           iApply ("H" $! (Some _)).
-          iModIntro. simpl. iExists _. iSplit; [done|].
-          iRight. rewrite /auth_is_ser_3.
-          iExists _. iSplit; [done|].
-          eauto.
+          iModIntro. iExists _. iSplit; [done|].
+(*          { simpl. iExists _. iSplit; [done|].
+            iRight. rewrite /auth_is_ser_3.
+            iExists _, _. iSplit; [done|].
+            iInv "Hinv" as "[(%&%&%&%&Hser&HA&Hhash&#Hsusp)|(%&Hsusp)]" "Hclose".
+            iInv 
+            eauto. } *)
+          iRight. iExists _, _. iSplit; [done|].
+          iFrame. iSimpl. iLeft. done.
         * iModIntro. iApply ("H" $! (Some _)).
           iExists _. iSplit; [done|].
           iLeft. rewrite /auth_is_ser_1.
@@ -657,38 +1048,39 @@ Section proof.
       + by iApply ("H" $! None).
   Qed.
 
-  Lemma refines_auth_auth Θ (Δ : ctxO Σ Θ) R :
+  Lemma refines_auth_auth Θ (Δ : ctxO Σ Θ) R:
     ⊢ ⟦ ∀: ⋆, var1 var0 → var0 → var3 var0 ⟧
       (auth_ctx Δ R) v_auth i_auth.
   Proof.
     iIntros (???) "!# _"; rewrite -/interp.
-    iIntros (??) "Hi".
+    iIntros (??) "(Hi & Htok)".
     rewrite /v_auth  /i_auth.
     i_pures; wp_pures.
     iModIntro. iFrame. clear.
     iIntros (??) "!# #HeviA".
     rewrite /auth_ctx.
     interp_unfold! in "HeviA".
-    iDestruct "HeviA" as (tA ser count deser ->) "(#Hser & #Hcount & #Hdeser)".
-    iIntros (??) "Hi".
+    iDestruct "HeviA" as (tA ser count deser ->) "(#Hser & #Hser2 & #Hser3 & #Hcount & #Hdeser)".
+    iIntros (??) "(Hi & Htok)".
     i_pures; wp_pures.
     iFrame.
     interp_unfold.
     iIntros "!> !>" (w1 w2) "#HA". clear.
-    iIntros (??) "Hi".
+    iIntros (??) "(Hi & Htok)".
     i_pures; wp_pures.
     interp_unfold! in "HA".
-    wp_apply "Hser"; [done|].
-    iIntros (o) "#Hs1". destruct o; wp_pures; last first.
+    wp_apply ("Hser" with "[$Htok]"); [done|].
+    iIntros ([]) "(Htok & Hs1)"; wp_pures; last first.
     { iFrame. interp_unfold!. by iRight. }
     wp_apply (wp_hash with "[$]"). iIntros "#Hh1".
     wp_pures.
     iFrame.
     interp_unfold!.
     iLeft. iExists _.
-    iModIntro. iSplit; [done|]. iLeft.    
-    iExists _,_,_. 
-    by iFrame "# %".
+    iModIntro. iSplit; [done|].
+    iExists _, _, _. iFrame "# ∗ %".
+    by iLeft.
   Qed.
 
 End proof.
+
